theories/BWT/Sorting/Sort.v
@@ -1,0 +1,58 @@
+Require Import Coq.Sorting.Permutation.
+
+Require Import BWT.Sorting.Ord.
+Require Import BWT.Sorting.Sorted.
+Require Import BWT.Sorting.StablePerm.
+
+Section Sort.
+  Context {A : Type}.
+
+  Implicit Types (f g : list A -> list A).
+
+  Section Preord.
+    Context {O : Preord A}.
+
+    Definition Sort f :=
+      forall l, Sorted (f l) /\ Permutation (f l) l.
+
+    Definition StableSort f :=
+      forall l, Sorted (f l) /\ StablePerm (f l) l.
+
+    Remark StableSort_Sort : forall f,
+        StableSort f -> Sort f.
+    Proof.
+      intros f HF l; destruct (HF l).
+      split; [|apply StablePerm_Perm]; easy.
+    Qed.
+
+    Theorem StableSort_unique : forall f g,
+        StableSort f -> StableSort g ->
+        (forall l, f l = g l).
+    Proof.
+      intros f g HF HG l.
+      apply StablePerm_Sorted_eq; [apply HF|apply HG|].
+      transitivity l; [|symmetry]; [apply HF| apply HG].
+    Qed.
+  End Preord.
+
+  Section Leibniz.
+    Context `{O : Ord A}.
+
+    Theorem Sort_StableSort_Ord : forall f,
+        Sort f <-> StableSort f.
+    Proof.
+      split; [|apply StableSort_Sort].
+      intros HF.
+      split; [apply HF|].
+      apply all_perm_stable; [apply eqv_eq|apply HF].
+    Qed.
+
+    Theorem Sort_Ord_unique : forall f g,
+        Sort f -> Sort g ->
+        (forall l, f l = g l).
+    Proof.
+      setoid_rewrite Sort_StableSort_Ord.
+      exact StableSort_unique.
+    Qed.
+  End Leibniz.
+End Sort.
